src/program_proof/mpaxos/init_proof.v
@@ -3,9 +3,109 @@ From Goose.github_com.mit_pdos.gokv Require mpaxos.
 From Perennial.program_proof.grove_shared Require Import urpc_proof urpc_spec.
 From Perennial.program_proof.mpaxos Require Export definitions protocol_proof.
 
-Section start_proof.
-Context `{!heapGS Σ}.
+Section init_proof.
+Context `{!gooseGlobalGS Σ}.
 Context `{!mpG Σ}.
+
+Definition is_mpaxos_sys_init_witness γ config N : iProp Σ :=
+  is_sys_init_witness (config:=config) (N:=N) γ.(s_mp)
+.
+
+Definition is_mpaxos_server_prealloc_witness γsrv : iProp Σ :=
+  is_accepted_lb γsrv (U64 0) [].
+
+Lemma prealloc_mpaxos_server :
+  ⊢ |={⊤}=> ∃ γsrv,
+  is_mpaxos_server_prealloc_witness γsrv ∗
+  (∀ γ (p:mpaxosParams.t Σ),
+     is_mpaxos_sys_init_witness γ p.(mpaxosParams.config) p.(mpaxosParams.N) -∗
+        own_file_inv γ γsrv []).
+Proof.
+  (* iMod (pb_ghost_server_pre_init) as (γpb) "(Hpre & #? & #?)".
+  iMod (alloc_primary_protocol_server) as (γprim) "Hprim".
+  iExists {| r_pb := γpb ; r_prim := γprim |}.
+  iModIntro. iFrame "#".
+  iIntros (?) "#(? & ? & ?)".
+  iDestruct (pb_ghost_server_init with "[$] [$]") as "H".
+  by iExists _; iFrame "∗#". *)
+Admitted.
+
+(* Invariants:
+   is_repl_inv
+   is_vote_inv
+   is_helping_inv
+ *)
+
+Lemma alloc_mpaxos_helping_inv {p:mpaxosParams.t Σ} γ :
+  own_log γ.(s_mp) [] -∗ own_state γ p.(mpaxosParams.initstate)
+  ={⊤}=∗ is_helping_inv γ.
+Proof.
+  iIntros "Hprelog Hint_log".
+  iMod (inv_alloc with "[-]") as "$"; last done.
+  iNext.
+  iExists [].
+  iFrame.
+  iSplitL.
+  {
+    iExists [].
+    iFrame.
+    iSplitR; first done.
+    iApply big_sepL2_nil.
+    done.
+  }
+  iModIntro.
+  iIntros.
+  exfalso.
+  rewrite H0 in H.
+  apply prefix_nil_inv in H.
+  apply (f_equal length) in H.
+  rewrite app_length /= in H.
+  lia.
+Qed.
+
+Lemma alloc_mpaxos_system γsrvs init N Pwf :
+  length γsrvs > 0 →
+  (∀ γsrv, ⌜γsrv ∈ γsrvs⌝ → is_mpaxos_server_prealloc_witness γsrv)
+  ={⊤}=∗
+  let params:=(mpaxosParams.mk Σ γsrvs init Pwf N) in
+  ∃ γ,
+   is_helping_inv γ ∗
+   is_vote_inv (config:=γsrvs) (N:=N) γ.(s_mp) ∗
+   is_repl_inv (config:=γsrvs) (N:=N) γ.(s_mp) ∗
+   own_state γ init ∗
+   is_mpaxos_sys_init_witness γ γsrvs N
+.
+Proof.
+  (* iIntros (?) "#Hpre".
+  iMod alloc_primary_protocol as (γprim) "[Hprim #HprimWit]".
+  iMod (pb_system_init (r_pb <$> γsrvs) with "[]") as (γpb) "Hpb".
+  { by rewrite fmap_length. }
+  { iIntros.
+    apply elem_of_list_fmap_2 in H0 as (? & ? & ?); subst.
+    by iApply "Hpre". }
+  iDestruct "Hpb" as "(#Hrep & Hlog & Hinit & #Hwit)".
+  iMod (alloc_pb_preread_protocol with "Hlog") as (γprelog γreads) "[#Hpreread Hlog]".
+  iMod (own_alloc (●ML [])) as (γintlog) "[Hintlog Hintlog2]".
+  { apply mono_list_auth_valid. }
+  iMod (own_alloc (●ML [])) as (γoplog) "[Hoplog Hoplog2]".
+  { apply mono_list_auth_valid. }
+
+  set (γ:={| s_pb:=γpb ; s_prim:=γprim ; s_prelog := γprelog ; s_internal_log := γintlog ;
+             s_reads:=γreads ; s_log := γoplog
+          |}).
+  iMod (alloc_helping_inv γ with "Hlog Hintlog2") as "#Hhelp".
+  iAssert (|={⊤}=> is_proph_read_inv γ)%I with "[Hintlog Hoplog2]" as ">#Hproph_read_inv".
+  { iApply (inv_alloc with "[Hintlog Hoplog2]").
+    iExists _; iFrame. }
+  iModIntro. iExists γ.
+  iNamed "Hinit".
+  iFrame "∗ His_conf #".
+  iIntros.
+  iExists _; iFrame "#".
+  iPureIntro.
+  by apply elem_of_list_fmap_1. *)
+Admitted.
+
 Context `{Hparams:!mpaxosParams.t Σ}.
 Import mpaxosParams.
 
@@ -33,100 +133,4 @@ Proof.
   set_solver.
 Qed.
 
-Definition is_mpaxos_sys_init_witness γ : iProp Σ :=
-  is_sys_init_witness γ.(s_mp)
-.
-
-Definition is_mpaxos_server_prealloc_witness γsrv : iProp Σ :=
-  is_accepted_lb γsrv (U64 0) [].
-
-Lemma prealloc_mpaxos_server :
-  ⊢ |={⊤}=> ∃ γsrv,
-  is_mpaxos_server_prealloc_witness γsrv ∗
-  (∀ γ, is_mpaxos_sys_init_witness γ -∗
-        own_paxosState_ghost γ γsrv (paxosState.mk 0 0 0 initstate false)).
-Proof.
-  iMod (pb_ghost_server_pre_init) as (γpb) "(Hpre & #? & #?)".
-  iMod (alloc_primary_protocol_server) as (γprim) "Hprim".
-  iExists {| r_pb := γpb ; r_prim := γprim |}.
-  iModIntro. iFrame "#".
-  iIntros (?) "#(? & ? & ?)".
-  iDestruct (pb_ghost_server_init with "[$] [$]") as "H".
-  by iExists _; iFrame "∗#".
-Qed.
-
-(* Invariants:
-   is_repl_inv
-   is_helping_inv
- *)
-
-Lemma alloc_helping_inv γ :
-  own_pre_log γ.(s_prelog) [] -∗ own_int_log γ []
-  ={⊤}=∗ is_helping_inv γ.
-Proof.
-  iIntros "Hprelog Hint_log".
-  iMod (inv_alloc with "[-]") as "$"; last done.
-  iNext.
-  iExists [].
-  iFrame.
-  iSplitL.
-  {
-    iExists [].
-    iFrame.
-    iSplitR; first done.
-    iApply big_sepL2_nil.
-    done.
-  }
-  iModIntro.
-  iIntros.
-  exfalso.
-  rewrite H0 in H.
-  apply prefix_nil_inv in H.
-  apply (f_equal length) in H.
-  rewrite app_length /= in H.
-  lia.
-Qed.
-
-Lemma alloc_simplepb_system γsrvs :
-  length γsrvs > 0 →
-  (∀ γsrv, ⌜γsrv ∈ γsrvs⌝ → is_accepted_lb γsrv.(r_pb) (U64 0) [] ∗ is_epoch_lb γsrv.(r_pb) 0)
-  ={⊤}=∗ ∃ γ,
-  is_pb_system_invs γ ∗
-  own_op_log γ [] ∗
-  (∀ γsrv, ⌜γsrv ∈ γsrvs⌝ → is_pb_sys_init_witness γ γsrv) ∗
-  pb_init_for_config γ.(s_pb) (r_pb <$> γsrvs) ∗
-  primary_init_for_config γ.(s_prim) ∗
-  is_proph_read_inv γ
-.
-Proof.
-  iIntros (?) "#Hpre".
-  iMod alloc_primary_protocol as (γprim) "[Hprim #HprimWit]".
-  iMod (pb_system_init (r_pb <$> γsrvs) with "[]") as (γpb) "Hpb".
-  { by rewrite fmap_length. }
-  { iIntros.
-    apply elem_of_list_fmap_2 in H0 as (? & ? & ?); subst.
-    by iApply "Hpre". }
-  iDestruct "Hpb" as "(#Hrep & Hlog & Hinit & #Hwit)".
-  iMod (alloc_pb_preread_protocol with "Hlog") as (γprelog γreads) "[#Hpreread Hlog]".
-  iMod (own_alloc (●ML [])) as (γintlog) "[Hintlog Hintlog2]".
-  { apply mono_list_auth_valid. }
-  iMod (own_alloc (●ML [])) as (γoplog) "[Hoplog Hoplog2]".
-  { apply mono_list_auth_valid. }
-
-  set (γ:={| s_pb:=γpb ; s_prim:=γprim ; s_prelog := γprelog ; s_internal_log := γintlog ;
-             s_reads:=γreads ; s_log := γoplog
-          |}).
-  iMod (alloc_helping_inv γ with "Hlog Hintlog2") as "#Hhelp".
-  iAssert (|={⊤}=> is_proph_read_inv γ)%I with "[Hintlog Hoplog2]" as ">#Hproph_read_inv".
-  { iApply (inv_alloc with "[Hintlog Hoplog2]").
-    iExists _; iFrame. }
-  iModIntro. iExists γ.
-  iNamed "Hinit".
-  iFrame "∗ His_conf #".
-  iIntros.
-  iExists _; iFrame "#".
-  iPureIntro.
-  by apply elem_of_list_fmap_1.
-Qed.
-
-End pb_init_proof.
+End init_proof.
